src/Notations.v
@@ -16,19 +16,20 @@
 (** printing =] $\sqsupseteq$ *)
 (** printing == $\equiv$ *)
 
-Reserved Notation "x * y" (at level 40, left associativity).
-Reserved Notation "x ** y" (at level 40, left associativity).
 Reserved Notation "x 'o' y" (at level 30, right associativity).
-Reserved Notation "x || y" (at level 50, left associativity).
+Reserved Notation "x ^^ n" (at level 38, left associativity).
+Reserved Notation "x ** y" (at level 39, left associativity).
+Reserved Notation "x * y" (at level 40, left associativity).
 Reserved Notation "x (+) y" (at level 45, no associativity).
+Reserved Notation "x || y" (at level 50, left associativity).
 Reserved Notation "x --> y" (at level 55, right associativity).
 Reserved Notation "x @ f" (at level 55, right associativity).
+Reserved Notation "\ x , y" (at level 58, right associativity).
+Reserved Notation "\\ x , y ; z" (at level 59, right associativity).
 Reserved Notation "x [= y" (at level 60, no associativity).
 Reserved Notation "x [!= y" (at level 60, no associativity).
 Reserved Notation "x == y" (at level 60, no associativity).
 Reserved Notation "x ->> y" (at level 60, no associativity).
-Reserved Notation "\ x , y" (at level 58, right associativity).
-Reserved Notation "\\ x , y ; z" (at level 59, right associativity).
 
 Reserved Notation "[ x ]".
 
